Standard semantics

deep/Small.v
@@ -8,17 +8,10 @@ Require Export Classical.
 
 Require Import OnSeparationLogic.StrongInduction.
 
-Module Type AbstractSemantics.
+Section ProgramSignature.
 
-Parameter op: Type.
-Parameter test: Type.
-Parameter state: Type.
-Parameter op_interp: op -> state -> option (state -> Prop).
-Parameter test_interp: test -> state -> Prop.
-
-End AbstractSemantics.
-
-Module AbstractSemanticsFacts (Import AS: AbstractSemantics).
+Variable op: Type.
+Variable test: Type.
 
 Inductive program :=
 | oper: op -> program
@@ -33,41 +26,6 @@ Inductive continuation :=
 | done: continuation
 | next: program -> continuation.
 Coercion next: program >-> continuation.
-
-Inductive configuration :=
-| continue: continuation -> state -> configuration
-| failure: configuration.
-
-Inductive smallstep: configuration -> configuration -> Prop :=
-| sstep_oper (O: op) (s s': state) (X: state -> Prop):
-    op_interp O s = Some X /\ X s' ->
-    smallstep (continue O s) (continue done s')
-| sstep_oper_fail (O: op) (s: state):
-    op_interp O s = None ->
-    smallstep (continue O s) failure
-| sstep_skip (s: state):
-    smallstep (continue skip s) (continue done s)
-| sstep_comp1 (S1 S1' S2: program) (s s': state):
-    smallstep (continue S1 s) (continue S1' s') ->
-    smallstep (continue (comp S1 S2) s) (continue (comp S1' S2) s')
-| sstep_comp2 (S1 S2: program) (s s': state):
-    smallstep (continue S1 s) (continue done s') ->
-    smallstep (continue (comp S1 S2) s) (continue S2 s')
-| sstep_comp_fail (S1 S2: program) (s: state):
-    smallstep (continue S1 s) failure ->
-    smallstep (continue (comp S1 S2) s) failure
-| sstep_ite_true (T: test) (S1 S2: program) (s: state):
-    test_interp T s ->
-    smallstep (continue (ite T S1 S2) s) (continue S1 s)
-| sstep_ite_false (T: test) (S1 S2: program) (s: state):
-    ~test_interp T s ->
-    smallstep (continue (ite T S1 S2) s) (continue S2 s)
-| sstep_while_true (T: test) (S: program) (s: state):
-    test_interp T s ->
-    smallstep (continue (while T S) s) (continue (comp S (while T S)) s)
-| sstep_while_false (T: test) (S: program) (s: state):
-    ~test_interp T s ->
-    smallstep (continue (while T S) s) (continue done s).
 
 Inductive context :=
 | hole: context
@@ -104,6 +62,67 @@ Proposition prime_prime_context (S: program):
 induction S; auto.
 simpl. rewrite IHS1. auto.
 Qed.
+
+Fixpoint remainder (S: program): continuation :=
+match S with
+| comp S1 S2 => match (remainder S1) with
+                | done => S2
+                | next S1 => comp S1 S2
+                end
+| _ => done
+end.
+
+Definition plug_remainder (C1: continuation) (S2: program): continuation :=
+match C1 with
+| done => remainder S2
+| next S1 => (plug (prime_context S2) S1)
+end.
+
+Record machine_model (mstate: Type) :=
+{ mop_interp: op -> mstate -> option (mstate -> Prop)
+; mtest_interp: test -> mstate -> Prop }.
+
+Section AbstractSemantics.
+
+Context {state: Type}.
+Variable M: machine_model state.
+Definition op_interp (o: op) (s: state) := mop_interp state M o s.
+Definition test_interp (t: test) (s: state) := mtest_interp state M t s.
+
+Inductive configuration :=
+| continue: continuation -> state -> configuration
+| failure: configuration.
+
+Inductive smallstep: configuration -> configuration -> Prop :=
+| sstep_oper (O: op) (s s': state) (X: state -> Prop):
+    op_interp O s = Some X /\ X s' ->
+    smallstep (continue O s) (continue done s')
+| sstep_oper_fail (O: op) (s: state):
+    op_interp O s = None ->
+    smallstep (continue O s) failure
+| sstep_skip (s: state):
+    smallstep (continue skip s) (continue done s)
+| sstep_comp1 (S1 S1' S2: program) (s s': state):
+    smallstep (continue S1 s) (continue S1' s') ->
+    smallstep (continue (comp S1 S2) s) (continue (comp S1' S2) s')
+| sstep_comp2 (S1 S2: program) (s s': state):
+    smallstep (continue S1 s) (continue done s') ->
+    smallstep (continue (comp S1 S2) s) (continue S2 s')
+| sstep_comp_fail (S1 S2: program) (s: state):
+    smallstep (continue S1 s) failure ->
+    smallstep (continue (comp S1 S2) s) failure
+| sstep_ite_true (T: test) (S1 S2: program) (s: state):
+    test_interp T s ->
+    smallstep (continue (ite T S1 S2) s) (continue S1 s)
+| sstep_ite_false (T: test) (S1 S2: program) (s: state):
+    ~test_interp T s ->
+    smallstep (continue (ite T S1 S2) s) (continue S2 s)
+| sstep_while_true (T: test) (S: program) (s: state):
+    test_interp T s ->
+    smallstep (continue (while T S) s) (continue (comp S (while T S)) s)
+| sstep_while_false (T: test) (S: program) (s: state):
+    ~test_interp T s ->
+    smallstep (continue (while T S) s) (continue done s).
 
 Lemma smallstep_prime (S S': program) (s s': state):
   smallstep (continue (prime S) s) (continue S' s') ->
@@ -144,15 +163,6 @@ simpl in H. apply smallstep_comp_diverge.
 apply IHS1. apply H.
 Qed.
 
-Fixpoint remainder (S: program): continuation :=
-match S with
-| comp S1 S2 => match (remainder S1) with
-                | done => S2
-                | next S1 => comp S1 S2
-                end
-| _ => done
-end.
-
 Lemma smallstep_remainder (S: program) (s s': state):
   smallstep (continue (prime S) s) (continue done s') ->
   smallstep (continue S s) (continue (remainder S) s').
@@ -164,12 +174,6 @@ destruct (remainder S1).
 apply sstep_comp2. apply IHS1. apply H.
 apply sstep_comp1. apply IHS1. apply H.
 Qed.
-
-Definition plug_remainder (C1: continuation) (S2: program): continuation :=
-match C1 with
-| done => remainder S2
-| next S1 => (plug (prime_context S2) S1)
-end.
 
 Lemma smallstep_plug_remainder (S: program) (CC: continuation) (s s': state):
   smallstep (continue (prime S) s) (continue CC s') ->
@@ -728,3 +732,899 @@ induction x; intros.
   + apply IHx in H2.
     eapply smallstep_bigstep. apply H1. apply H2.
 Qed.
+
+Definition resultset := option state -> Prop.
+Definition stateset := state -> Prop.
+
+Definition stateset_to_resultset (X: stateset): resultset :=
+fun os => exists s, os = Some s /\ X s.
+Coercion stateset_to_resultset: stateset >-> resultset.
+
+Definition bigstep_initial_resultset (I: configuration): resultset :=
+fun os => match os with
+| None => bigstep I failure
+| Some s => bigstep I (continue done s)
+end.
+
+Definition bigstep_program_resultset (S: program) (os: option state): resultset :=
+match os with
+| None => fun os' => os' = None
+| Some s => bigstep_initial_resultset (continue S s)
+end.
+
+Definition bigstep_denotation (S: program) (Y: resultset): resultset :=
+fun os => forall y, Y y -> (bigstep_program_resultset S y) os.
+
+Definition compose {A: Type} (f g: A -> A): A -> A := fun x => f (g x).
+
+Definition cap_fail (Y: resultset): resultset :=
+fun os => Y os /\ os = None.
+Definition cap_state (Y: resultset) (X: state -> Prop): resultset :=
+fun os => Y os /\ forall s, os = Some s -> X s.
+Definition complement (X: state -> Prop): state -> Prop :=
+fun s => ~X s.
+
+Fixpoint approx_denotation (n: nat): program -> resultset -> resultset :=
+fix approx_denotation_prog (S: program) :=
+  match S with
+  | oper o => fun Y os =>
+      cap_fail Y os \/
+      (exists s, Y (Some s) /\ op_interp o s = None /\ os = None) \/
+      (exists s X s', Y (Some s) /\ op_interp o s = Some X /\ os = Some s' /\ X s')
+  | skip => id
+  | diverge => cap_fail
+  | comp S1 S2 => compose (approx_denotation_prog S2) (approx_denotation_prog S1)
+  | ite T S1 S2 => fun Y os =>
+      cap_fail Y os \/
+      (approx_denotation_prog S1 (cap_state Y (test_interp T)) os) \/
+      (approx_denotation_prog S2 (cap_state Y (complement (test_interp T))) os)
+  | while T S1 =>
+      match n with
+      | O => cap_fail
+      | S n => approx_denotation n (ite T (comp S1 (while T S1)) skip)
+      end
+  end.
+Proposition approx_denotation_comp (n: nat) (S1 S2: program):
+  approx_denotation n (comp S1 S2) = compose (approx_denotation n S2) (approx_denotation n S1).
+destruct n; reflexivity.
+Qed.
+Proposition approx_denotation_ite (n: nat) (T: test) (S1 S2: program) (Y: resultset):
+  approx_denotation n (ite T S1 S2) Y =
+  fun os => (cap_fail Y os) \/
+    (approx_denotation n S1 (cap_state Y (test_interp T)) os) \/
+    (approx_denotation n S2 (cap_state Y (complement (test_interp T))) os).
+destruct n.
+apply functional_extensionality; intros.
+apply propositional_extensionality.
+simpl.
+apply or_iff_compat_l.
+apply ZifyClasses.or_morph.
+apply iff_refl.
+apply iff_refl.
+apply functional_extensionality; intros.
+apply propositional_extensionality.
+simpl.
+apply or_iff_compat_l.
+apply ZifyClasses.or_morph.
+apply iff_refl.
+apply iff_refl.
+Qed.
+Proposition approx_denotation_while (n: nat) (T: test) (S1: program):
+  approx_denotation (S n) (while T S1) = approx_denotation n (ite T (comp S1 (while T S1)) skip).
+reflexivity.
+Qed.
+
+Lemma approx_monotonic (n: nat) (S1: program) (X Y: resultset):
+  (forall os, X os -> Y os) ->
+  forall os, approx_denotation n S1 X os -> approx_denotation n S1 Y os.
+intros. generalize dependent Y. generalize dependent X. generalize dependent os. generalize dependent S1. induction n; intros.
+- generalize dependent Y. generalize dependent X. generalize dependent os. induction S1; intros.
+  + simpl in *. destruct H0.
+    left. unfold cap_fail in *. destruct H0. constructor; auto.
+    right. destruct H0.
+    left. destruct H0. exists x. destruct H0. destruct H1. constructor; auto.
+    right. destruct H0. destruct H0. destruct H0. destruct H0. destruct H1. destruct H2.
+    exists x. exists x0. exists x1. constructor; auto.
+  + simpl in *. unfold cap_fail in *. destruct H0. constructor; auto.
+  + simpl in *. unfold id in *. auto.
+  + rewrite approx_denotation_comp in H0.
+    rewrite approx_denotation_comp.
+    unfold compose in *.
+    eapply IHS1_2. apply H0. intros.
+    eapply IHS1_1. apply H1. apply H.
+  + rewrite approx_denotation_ite in H0.
+    rewrite approx_denotation_ite.
+    destruct H0. left. unfold cap_fail in *. destruct H0. constructor; auto.
+    destruct H0. right. left.
+    eapply IHS1_1. apply H0. intros.
+    unfold cap_state in *. destruct H1. constructor; auto.
+    right. right. eapply IHS1_2. apply H0.
+    intros. unfold cap_state in *. destruct H1. constructor; auto.
+  + unfold approx_denotation in H0. unfold cap_fail in H0.
+    unfold approx_denotation. unfold cap_fail. destruct H0. constructor; auto.
+- generalize dependent Y. generalize dependent X. generalize dependent os. induction S1; intros.
+  + simpl in *. destruct H0.
+    left. unfold cap_fail in *. destruct H0. constructor; auto.
+    right. destruct H0.
+    left. destruct H0. exists x. destruct H0. destruct H1. constructor; auto.
+    right. destruct H0. destruct H0. destruct H0. destruct H0. destruct H1. destruct H2.
+    exists x. exists x0. exists x1. constructor; auto.
+  + simpl in *. unfold cap_fail in *. destruct H0. constructor; auto.
+  + simpl in *. unfold id in *. auto.
+  + rewrite approx_denotation_comp in H0.
+    rewrite approx_denotation_comp.
+    unfold compose in *.
+    eapply IHS1_2. apply H0. intros.
+    eapply IHS1_1. apply H1. apply H.
+  + rewrite approx_denotation_ite in H0.
+    rewrite approx_denotation_ite.
+    destruct H0. left. unfold cap_fail in *. destruct H0. constructor; auto.
+    destruct H0. right. left.
+    eapply IHS1_1. apply H0. intros.
+    unfold cap_state in *. destruct H1. constructor; auto.
+    right. right. eapply IHS1_2. apply H0.
+    intros. unfold cap_state in *. destruct H1. constructor; auto.
+  + rewrite approx_denotation_while in H0.
+    rewrite approx_denotation_while.
+    eapply IHn. apply H0. apply H.
+Qed.
+
+Lemma approximation (n: nat) (S1: program) (Y: resultset):
+  forall os, approx_denotation n S1 Y os -> approx_denotation (S n) S1 Y os.
+intros. generalize dependent S1. generalize dependent os. generalize dependent Y. induction n; intros.
+- generalize dependent os. generalize dependent Y. induction S1; intros; auto.
+  + rewrite approx_denotation_comp in H.
+    rewrite approx_denotation_comp.
+    unfold compose in *.
+    apply IHS1_2.
+    eapply approx_monotonic; [|apply H].
+    apply IHS1_1.
+  + rewrite approx_denotation_ite in H.
+    rewrite approx_denotation_ite.
+    destruct H. left; auto.
+    destruct H; right.
+    left. apply IHS1_1. auto.
+    right. apply IHS1_2. auto.
+  + simpl in H. unfold approx_denotation; left. auto.
+- generalize dependent os. generalize dependent Y. induction S1; intros; auto.
+  + rewrite approx_denotation_comp in H.
+    rewrite approx_denotation_comp.
+    unfold compose in *.
+    apply IHS1_2.
+    eapply approx_monotonic; [|apply H].
+    apply IHS1_1.
+  + rewrite approx_denotation_ite in H.
+    rewrite approx_denotation_ite.
+    destruct H. left; auto.
+    destruct H; right.
+    left. apply IHS1_1. auto.
+    right. apply IHS1_2. auto.
+  + rewrite approx_denotation_while in H.
+    rewrite approx_denotation_while.
+    apply IHn. auto.
+Qed.
+
+Corollary approximation_le (n m: nat) (S1: program) (Y: resultset):
+  n <= m -> forall os, approx_denotation n S1 Y os -> approx_denotation m S1 Y os.
+intro. induction m.
+- inversion H. auto.
+- inversion H. auto.
+  intros.
+  apply approximation.
+  apply IHm; auto.
+Qed.
+
+Proposition approx_comp (n m: nat) (S1 S2: program) (X: resultset) (os: option state):
+  approx_denotation n S2 (approx_denotation m S1 X) os ->
+  approx_denotation (max n m) (comp S1 S2) X os.
+intros.
+generalize dependent os.
+generalize dependent X.
+generalize dependent S2.
+generalize dependent S1.
+generalize dependent m.
+induction n; intros.
+- simpl. rewrite approx_denotation_comp.
+  unfold compose.
+  apply approximation_le with (n := 0).
+  apply Nat.le_0_l. auto.
+- rewrite approx_denotation_comp.
+  unfold compose.
+  destruct m.
+  + rewrite Nat.max_0_r.
+    eapply approx_monotonic; [|apply H].
+    intros. apply approximation_le with (n := 0).
+    apply Nat.le_0_l. auto.
+  + rewrite <- Nat.succ_max_distr.
+    generalize dependent os.
+    generalize dependent X.
+    generalize dependent S1.
+    generalize dependent n.
+    generalize dependent m.
+    induction S2; intros.
+    * unfold approx_denotation at 1.
+      unfold approx_denotation in H at 1.
+      destruct H. left. unfold cap_fail in *.
+      destruct H. constructor.
+      eapply approximation_le; [|apply H].
+      apply Peano.le_n_S.
+      apply Nat.le_max_r. auto.
+      right. destruct H. left.
+      destruct H. exists x. destruct H.
+      constructor.
+      eapply approximation_le; [|apply H].
+      apply Peano.le_n_S.
+      apply Nat.le_max_r. auto.
+      right. destruct H. destruct H. destruct H. destruct H.
+      exists x. exists x0. exists x1. constructor.
+      eapply approximation_le; [|apply H].
+      apply Peano.le_n_S.
+      apply Nat.le_max_r. auto.
+    * unfold approx_denotation at 1.
+      unfold approx_denotation in H at 1.
+      unfold cap_fail in *. destruct H. constructor; auto.
+      eapply approximation_le; [|apply H].
+      apply Peano.le_n_S.
+      apply Nat.le_max_r.
+    * unfold approx_denotation at 1.
+      unfold approx_denotation in H at 1.
+      unfold id in *.
+      eapply approximation_le; [|apply H].
+      apply Peano.le_n_S.
+      apply Nat.le_max_r.
+    * rewrite approx_denotation_comp.
+      rewrite approx_denotation_comp in H.
+      unfold compose in *.
+      apply approx_monotonic with (Y := (approx_denotation (S (max n m)) S2_1 (approx_denotation (S m) S1 X))) in H.
+      **  apply IHS2_2 in H; auto.
+          rewrite Nat.max_assoc in H.
+          rewrite Nat.max_id in H.
+          eapply approx_monotonic; [|apply H].
+          intros.
+          eapply approx_monotonic; [|apply H0].
+          intros.
+          eapply approximation_le; [|apply H1].
+          apply Peano.le_n_S.
+          apply Nat.le_max_r.
+      **  intros.
+          eapply approximation_le; [|apply H0].
+          apply Peano.le_n_S.
+          apply Nat.le_max_l.
+    * rewrite approx_denotation_ite.
+      rewrite approx_denotation_ite in H. destruct H.
+      left. unfold cap_fail in *.
+      destruct H. constructor; auto.
+      eapply approximation_le; [|apply H].
+      apply Peano.le_n_S.
+      apply Nat.le_max_r.
+      destruct H. right. left.
+      apply approx_monotonic with (Y := (cap_state (approx_denotation (S (max n m)) S1 X) (test_interp t))) in H.
+      eapply approximation_le; [|apply H].
+      apply Peano.le_n_S.
+      apply Nat.le_max_l.
+      intros. unfold cap_state in H0. unfold cap_state. destruct H0.
+      constructor.
+      eapply approximation_le; [|apply H0].
+      apply Peano.le_n_S.
+      apply Nat.le_max_r. auto.
+      right. right.
+      apply approx_monotonic with (Y := (cap_state (approx_denotation (S (max n m)) S1 X) (complement (test_interp t)))) in H.
+      eapply approximation_le; [|apply H].
+      apply Peano.le_n_S.
+      apply Nat.le_max_l.
+      intros. unfold cap_state in H0. unfold cap_state. destruct H0.
+      constructor.
+      eapply approximation_le; [|apply H0].
+      apply Peano.le_n_S.
+      apply Nat.le_max_r. auto.
+    * rewrite approx_denotation_while in H.
+      rewrite approx_denotation_while.
+      rewrite approx_denotation_ite.
+      rewrite approx_denotation_ite in H. destruct H.
+      left. unfold cap_fail in *.
+      destruct H. constructor; auto.
+      eapply approximation_le; [|apply H].
+      apply Peano.le_n_S.
+      apply Nat.le_max_r.
+      right. destruct H; [left|right].
+      apply approx_monotonic with (Y := (cap_state (approx_denotation (S (Nat.max n m)) S1 X) (test_interp t))) in H.
+      eapply approximation_le; [|apply H].
+      apply Nat.le_max_l.
+      intros. unfold cap_state in H0. unfold cap_state. destruct H0.
+      constructor. eapply approximation_le; [|apply H0].
+      apply Peano.le_n_S.
+      apply Nat.le_max_r. auto.
+      apply approx_monotonic with (Y := (cap_state (approx_denotation (S (Nat.max n m)) S1 X) (complement (test_interp t)))) in H.
+      eapply approximation_le; [|apply H].
+      apply Nat.le_max_l.
+      intros. unfold cap_state in H0. unfold cap_state. destruct H0.
+      constructor. eapply approximation_le; [|apply H0].
+      apply Peano.le_n_S.
+      apply Nat.le_max_r. auto.
+Qed.
+
+Definition denotation (S1: program): resultset -> resultset :=
+fun Y os => exists n, approx_denotation n S1 Y os.
+
+Lemma denotation_monotonic (S1: program) (X Y: resultset):
+  (forall os, X os -> Y os) ->
+  forall os, denotation S1 X os -> denotation S1 Y os.
+intros. unfold denotation in H0. unfold denotation.
+destruct H0. exists x.
+eapply approx_monotonic; [|apply H0].
+auto.
+Qed.
+
+Proposition denotation_oper (o: op):
+  denotation (oper o) = (fun Y os =>
+      cap_fail Y os \/
+      (exists s, Y (Some s) /\ op_interp o s = None /\ os = None) \/
+      (exists s X s', Y (Some s) /\ op_interp o s = Some X /\ os = Some s' /\ X s')).
+unfold denotation. unfold approx_denotation.
+apply functional_extensionality; intro.
+apply functional_extensionality; intro.
+apply propositional_extensionality.
+split; intro. destruct H. destruct x1; auto.
+exists 0. auto.
+Qed.
+
+Proposition denotation_skip:
+  denotation skip = id.
+unfold denotation. unfold approx_denotation.
+apply functional_extensionality; intro.
+apply functional_extensionality; intro.
+apply propositional_extensionality.
+split; intro. destruct H. destruct x1; auto.
+exists 0. auto.
+Qed.
+
+Proposition denotation_diverge:
+  denotation diverge = cap_fail.
+unfold denotation. unfold approx_denotation.
+apply functional_extensionality; intro.
+apply functional_extensionality; intro.
+apply propositional_extensionality.
+split; intro. destruct H. destruct x1; auto.
+exists 0. auto.
+Qed.
+
+Proposition approx_assoc (n: nat) (S1 S2 S3: program) (X: resultset):
+  approx_denotation n (comp (comp S1 S2) S3) X =
+  approx_denotation n (comp S1 (comp S2 S3)) X.
+rewrite approx_denotation_comp.
+rewrite approx_denotation_comp.
+rewrite approx_denotation_comp.
+rewrite approx_denotation_comp.
+unfold compose.
+reflexivity.
+Qed.
+
+Proposition denotation_assoc (S1 S2 S3: program) (X: resultset):
+  denotation (comp (comp S1 S2) S3) X =
+  denotation (comp S1 (comp S2 S3)) X.
+unfold denotation.
+apply functional_extensionality; intro os.
+apply propositional_extensionality; split; intro; destruct H; exists x.
+rewrite <- approx_assoc. auto.
+rewrite approx_assoc. auto.
+Qed.
+
+Definition assert (T: test): program := ite T skip diverge.
+Definition assert_not (T: test): program := ite T diverge skip.
+
+Proposition approx_fail (n: nat) (S1: program) (X: resultset):
+  X None -> approx_denotation n S1 X None.
+intros.
+generalize dependent X.
+generalize dependent S1.
+induction n; intro.
+- induction S1; intros.
+  + unfold approx_denotation. left. unfold cap_fail. auto.
+  + unfold approx_denotation. unfold cap_fail. auto.
+  + unfold approx_denotation. unfold id. auto.
+  + rewrite approx_denotation_comp. unfold compose.
+    apply IHS1_2. apply IHS1_1. auto.
+  + rewrite approx_denotation_ite. left. unfold cap_fail. auto.
+  + unfold approx_denotation. unfold cap_fail. auto.
+- induction S1; intros.
+  + unfold approx_denotation. left. unfold cap_fail. auto.
+  + unfold approx_denotation. unfold cap_fail. auto.
+  + unfold approx_denotation. unfold id. auto.
+  + rewrite approx_denotation_comp. unfold compose.
+    apply IHS1_2. apply IHS1_1. auto.
+  + rewrite approx_denotation_ite. left. unfold cap_fail. auto.
+  + rewrite approx_denotation_while.
+    apply IHn. auto.
+Qed.
+
+Proposition denotation_assert (T: test) (S: program) (X: resultset) (os: option state):
+  (cap_state (denotation S X) (test_interp T)) os -> (denotation (comp S (assert T)) X) os.
+unfold denotation in *; unfold cap_state in *; intros.
+destruct H. destruct H. exists x.
+rewrite approx_denotation_comp. unfold compose.
+unfold assert. rewrite approx_denotation_ite.
+right. left. unfold approx_denotation at 1; destruct x; unfold id;
+unfold cap_state; auto.
+Qed.
+
+Proposition denotation_assert_not (T: test) (S: program) (X: resultset) (os: option state):
+  (cap_state (denotation S X) (complement (test_interp T))) os -> (denotation (comp S (assert_not T)) X) os.
+unfold denotation in *; unfold cap_state in *; intros.
+destruct H. destruct H. exists x.
+rewrite approx_denotation_comp. unfold compose.
+unfold assert_not. rewrite approx_denotation_ite.
+right. right. unfold approx_denotation at 1; destruct x; unfold id;
+unfold cap_state; auto.
+Qed.
+
+Proposition approx_ite_comp (n: nat) (T: test) (S1 S2 S3: program) (X: resultset) (os: option state):
+  approx_denotation n (ite T S1 S2) (denotation S3 X) os ->
+    approx_denotation n S1 (denotation (comp S3 (assert T)) X) os \/
+    approx_denotation n S2 (denotation (comp S3 (assert_not T)) X) os.
+intro.
+rewrite approx_denotation_ite in H.
+destruct H.
+unfold cap_fail in H. destruct H. rewrite H0 in *. clear dependent H0.
+left. apply approx_fail. unfold denotation in H. destruct H.
+unfold denotation. exists x. rewrite approx_denotation_comp. unfold compose.
+apply approx_fail. auto.
+destruct H; [left|right].
+eapply approx_monotonic; [intros|apply H].
+apply denotation_assert in H0. auto.
+eapply approx_monotonic; [intros|apply H].
+apply denotation_assert_not in H0. auto.
+Qed.
+
+Proposition approx_comp_ite_left (n: nat) (T: test) (S1 S2 S3: program) (X: resultset) (os: option state):
+  approx_denotation n (comp (comp S1 (assert T)) S2) X os ->
+  approx_denotation n (comp S1 (ite T S2 S3)) X os.
+intros.
+rewrite approx_denotation_comp in H.
+rewrite approx_denotation_comp.
+unfold compose in *.
+rewrite approx_denotation_ite.
+right. left.
+eapply approx_monotonic; [intros|apply H].
+rewrite approx_denotation_comp in H0.
+unfold compose in H0.
+unfold assert in H0.
+rewrite approx_denotation_ite in H0.
+destruct H0. unfold cap_fail in H0. destruct H0. rewrite H1.
+unfold cap_state. constructor. rewrite H1 in H0; auto. intros. inversion H2.
+destruct H0.
+unfold approx_denotation in H0 at 1; destruct n; unfold id in H0; auto.
+unfold approx_denotation in H0 at 1; destruct n; unfold cap_fail in H0. destruct H0.
+unfold cap_state in H0. destruct H0.
+unfold cap_state. constructor; auto. intros. rewrite H1 in H3. inversion H3.
+unfold cap_state in H0. destruct H0. destruct H0.
+unfold cap_state. constructor; auto. intros. rewrite H1 in H3. inversion H3.
+Qed.
+
+Proposition approx_comp_ite_right (n: nat) (T: test) (S1 S2 S3: program) (X: resultset) (os: option state):
+  approx_denotation n (comp (comp S1 (assert_not T)) S3) X os ->
+  approx_denotation n (comp S1 (ite T S2 S3)) X os.
+intros.
+rewrite approx_denotation_comp in H.
+rewrite approx_denotation_comp.
+unfold compose in *.
+rewrite approx_denotation_ite.
+right. right.
+eapply approx_monotonic; [intros|apply H].
+rewrite approx_denotation_comp in H0.
+unfold compose in H0.
+unfold assert_not in H0.
+rewrite approx_denotation_ite in H0.
+destruct H0. unfold cap_fail in H0. destruct H0. rewrite H1.
+unfold cap_state. constructor. rewrite H1 in H0; auto. intros. inversion H2.
+destruct H0.
+unfold approx_denotation in H0 at 1; destruct n; unfold cap_fail in H0. destruct H0.
+unfold cap_state in H0. destruct H0.
+unfold cap_state. constructor; auto. intros. rewrite H1 in H3. inversion H3.
+unfold cap_state in H0. destruct H0. destruct H0.
+unfold cap_state. constructor; auto. intros. rewrite H1 in H3. inversion H3.
+unfold approx_denotation in H0 at 1; destruct n; unfold id in H0; auto.
+Qed.
+
+(* Proposition approx_fail (n: nat) (S1: program) (X: resultset): *)
+
+Lemma denotation_comp (S1 S2: program):
+  denotation (comp S1 S2) = compose (denotation S2) (denotation S1).
+unfold compose.
+apply functional_extensionality; intro.
+apply functional_extensionality; intro.
+apply propositional_extensionality.
+unfold denotation.
+split; intro.
+- destruct H.
+  exists x1.
+  rewrite approx_denotation_comp in H.
+  unfold compose in H.
+  eapply approx_monotonic; [|apply H].
+  intros.
+  exists x1. auto.
+- destruct H.
+  generalize dependent x0.
+  generalize dependent x.
+  generalize dependent S1.
+  generalize dependent S2.
+  induction x1; intro.
+  + induction S2; intros.
+    * unfold approx_denotation in H at 1. destruct H.
+      unfold cap_fail in H. destruct H. destruct H.
+      exists x1. rewrite approx_denotation_comp. unfold compose.
+      unfold approx_denotation at 1. destruct x1; left.
+      unfold cap_fail. auto. unfold cap_fail. auto.
+      destruct H. destruct H. destruct H. destruct H.
+      exists x2. rewrite approx_denotation_comp. unfold compose.
+      unfold approx_denotation at 1.
+      destruct x2; right; left; exists x1; constructor; auto.
+      destruct H. destruct H. destruct H. destruct H. destruct H.
+      exists x4. rewrite approx_denotation_comp. unfold compose.
+      unfold approx_denotation at 1.
+      destruct x4; right; right; exists x1; exists x2; exists x3; constructor; auto.
+    * unfold approx_denotation in H at 1.
+      unfold cap_fail in H. destruct H. destruct H.
+      exists x1. rewrite approx_denotation_comp; unfold compose.
+      unfold approx_denotation at 1. destruct x1; unfold cap_fail; auto.
+    * unfold approx_denotation in H at 1.
+      unfold id in H. destruct H.
+      exists x1. rewrite approx_denotation_comp; unfold compose.
+      unfold approx_denotation at 1. destruct x1; unfold id; auto.
+    * rewrite approx_denotation_comp in H. unfold compose in H.
+      apply approx_monotonic with (Y := fun os => (exists n : nat, approx_denotation n (comp S1 S2_1) x os)) in H.
+      enough (exists n : nat, approx_denotation n (comp (comp S1 S2_1) S2_2) x x0).
+      destruct H0. exists x1. rewrite <- approx_assoc. auto.
+      apply IHS2_2. auto.
+      intros. apply IHS2_1. auto.
+    * fold (denotation S1 x) in H. apply approx_ite_comp in H.
+      destruct H.
+      apply IHS2_1 in H. destruct H. exists x1.
+      apply approx_comp_ite_left. auto.
+      apply IHS2_2 in H. destruct H. exists x1.
+      apply approx_comp_ite_right. auto.
+    * unfold approx_denotation in H at 1. unfold cap_fail in H. destruct H. destruct H.
+      exists x1. rewrite approx_denotation_comp. unfold compose. rewrite H0. apply approx_fail.
+      rewrite H0 in H. auto.
+  + induction S2; intros.
+    * unfold approx_denotation in H at 1. destruct H.
+      unfold cap_fail in H. destruct H. destruct H.
+      exists x2. rewrite approx_denotation_comp. unfold compose.
+      unfold approx_denotation at 1. destruct x2; left.
+      unfold cap_fail. auto. unfold cap_fail. auto.
+      destruct H. destruct H. destruct H. destruct H.
+      exists x3. rewrite approx_denotation_comp. unfold compose.
+      unfold approx_denotation at 1.
+      destruct x3; right; left; exists x2; constructor; auto.
+      destruct H. destruct H. destruct H. destruct H. destruct H.
+      exists x5. rewrite approx_denotation_comp. unfold compose.
+      unfold approx_denotation at 1.
+      destruct x5; right; right; exists x2; exists x3; exists x4; constructor; auto.
+    * unfold approx_denotation in H at 1.
+      unfold cap_fail in H. destruct H. destruct H.
+      exists x2. rewrite approx_denotation_comp; unfold compose.
+      unfold approx_denotation at 1. destruct x2; unfold cap_fail; auto.
+    * unfold approx_denotation in H at 1.
+      unfold id in H. destruct H.
+      exists x2. rewrite approx_denotation_comp; unfold compose.
+      unfold approx_denotation at 1. destruct x2; unfold id; auto.
+    * rewrite approx_denotation_comp in H. unfold compose in H.
+      apply approx_monotonic with (Y := fun os => (exists n : nat, approx_denotation n (comp S1 S2_1) x os)) in H.
+      enough (exists n : nat, approx_denotation n (comp (comp S1 S2_1) S2_2) x x0).
+      destruct H0. exists x2. rewrite <- approx_assoc. auto.
+      apply IHS2_2. auto.
+      intros. apply IHS2_1. auto.
+    * fold (denotation S1 x) in H. apply approx_ite_comp in H.
+      destruct H.
+      apply IHS2_1 in H. destruct H. exists x2.
+      apply approx_comp_ite_left. auto.
+      apply IHS2_2 in H. destruct H. exists x2.
+      apply approx_comp_ite_right. auto.
+    * rewrite approx_denotation_while in H.
+      apply IHx1 in H. destruct H. exists (S x2).
+      rewrite approx_denotation_comp in H.
+      rewrite approx_denotation_comp.
+      unfold compose in *.
+      rewrite approx_denotation_while.
+      eapply approx_monotonic; [|apply H].
+      intros. apply approximation. auto.
+Qed.
+
+Proposition approx_skip (n: nat) (S1: program):
+  approx_denotation n S1 = approx_denotation n (comp skip S1).
+apply functional_extensionality; intro.
+rewrite approx_denotation_comp. unfold compose.
+unfold approx_denotation at 3. destruct n; unfold id; auto.
+Qed.
+
+Lemma denotation_ite (T: test) (S1 S2: program):
+  denotation (ite T S1 S2) = (fun X os => denotation (comp (assert T) S1) X os \/ denotation (comp (assert_not T) S2) X os).
+apply functional_extensionality; intro X.
+apply functional_extensionality; intro os.
+apply propositional_extensionality. split; intro.
+- unfold denotation in H. destruct H.
+  rewrite approx_denotation_ite in H. destruct H.
+  unfold cap_fail in H. destruct H.
+  left. unfold denotation. exists x.
+  rewrite approx_denotation_comp. unfold compose.
+  rewrite H0. apply approx_fail. apply approx_fail. rewrite <- H0. auto.
+  destruct H; [left|right].
+  + unfold denotation. exists x.
+    rewrite approx_denotation_comp. unfold compose.
+    eapply approx_monotonic; [intros|apply H].
+    unfold assert. rewrite approx_denotation_ite.
+    unfold cap_state in H0. destruct H0.
+    right. left.
+    unfold approx_denotation; destruct x; unfold id; unfold cap_state; auto.
+  + unfold denotation. exists x.
+    rewrite approx_denotation_comp. unfold compose.
+    eapply approx_monotonic; [intros|apply H].
+    unfold assert_not. rewrite approx_denotation_ite.
+    unfold cap_state in H0. destruct H0.
+    right. right.
+    unfold approx_denotation; destruct x; unfold id; unfold cap_state; auto.
+- destruct H; unfold denotation in H; destruct H.
+  unfold denotation; exists x.
+  rewrite approx_skip in H.
+  rewrite <- approx_assoc in H.
+  rewrite approx_skip.
+  apply approx_comp_ite_left. auto.
+  unfold denotation; exists x.
+  rewrite approx_skip in H.
+  rewrite <- approx_assoc in H.
+  rewrite approx_skip.
+  apply approx_comp_ite_right. auto.
+Qed.
+
+Fixpoint loop_unroll (k: nat) (T: test) (S1: program): program :=
+match k with
+| O => diverge
+| S k => ite T (comp S1 (loop_unroll k T S1)) skip
+end.
+
+Proposition iff_exists {T: Type} (P Q: T -> Prop):
+  (forall x, P x <-> Q x) ->
+  (exists x, P x) <-> (exists x, Q x).
+intros. split; intro; destruct H0; exists x; apply H; auto.
+Qed.
+
+Proposition compose_id_left {T: Type} (f: T -> T):
+  compose id f = f.
+apply functional_extensionality; intro x.
+unfold compose. unfold id. reflexivity.
+Qed.
+
+Lemma denotation_while (T: test) (S1: program):
+  denotation (while T S1) = (fun X os => exists k, denotation (loop_unroll k T S1) X os).
+apply functional_extensionality; intro X.
+apply functional_extensionality; intro os.
+apply propositional_extensionality.
+split; intro.
+- unfold denotation in H. destruct H.
+  generalize dependent X. generalize dependent os.
+  induction x; intros; simpl.
+  unfold approx_denotation in H.
+  exists 0. simpl. rewrite denotation_diverge. auto.
+  rewrite approx_denotation_while in H.
+  rewrite approx_denotation_ite in H. destruct H.
+  exists 0. simpl. rewrite denotation_diverge. auto.
+  destruct H.
+  + rewrite approx_denotation_comp in H. unfold compose in H.
+    apply IHx in H. destruct H. exists (S x0). simpl.
+    rewrite denotation_ite. left.
+    unfold denotation in H. destruct H.
+    unfold denotation.
+    apply approx_comp in H.
+    exists (max x1 x).
+    unfold assert.
+    rewrite approx_denotation_comp. unfold compose.
+    eapply approx_monotonic; [intros|apply H].
+    rewrite approx_denotation_ite. right. left.
+    unfold approx_denotation; destruct (max x1 x); unfold id; auto.
+  + unfold approx_denotation in H; destruct x; unfold id in H; exists 1; simpl;
+    unfold denotation; exists 0; rewrite approx_denotation_ite;
+    right; right; unfold approx_denotation; unfold id; auto.
+- destruct H.
+  unfold denotation in H. destruct H.
+  unfold denotation.
+  generalize dependent X. generalize dependent os.
+  induction x; intros.
+  simpl in H. exists 0. simpl. unfold approx_denotation in H. destruct x0; auto.
+  simpl in H. rewrite approx_denotation_ite in H. destruct H.
+  exists 0. simpl. auto. destruct H.
+  + rewrite approx_denotation_comp in H. unfold compose in H.
+    apply IHx in H. destruct H.
+    apply approx_comp in H.
+    exists (S (max x1 x0)).
+    rewrite approx_denotation_while.
+    rewrite approx_denotation_ite. right. left. auto.
+  + exists (S x0).
+    rewrite approx_denotation_while.
+    rewrite approx_denotation_ite. right. right. auto.
+Qed.
+
+Proposition denotation_while_compat (T: test) (S1 S2: program):
+  denotation S1 = denotation S2 ->
+  denotation (while T S1) = denotation (while T S2).
+intro.
+rewrite denotation_while.
+rewrite denotation_while.
+enough (forall k, denotation (loop_unroll k T S1) = denotation (loop_unroll k T S2)).
+{ apply functional_extensionality; intro X.
+apply functional_extensionality; intro os.
+apply propositional_extensionality.
+apply iff_exists. intro. rewrite H0. apply iff_refl. }
+intros. induction k; simpl. reflexivity.
+repeat rewrite denotation_ite.
+repeat rewrite denotation_comp.
+rewrite IHk. rewrite H. reflexivity.
+Qed.
+
+Lemma compositionality (S1 S2: program) (SC: context):
+  denotation S1 = denotation S2 ->
+  denotation (plug SC S1) = denotation (plug SC S2).
+intro. induction SC; simpl.
+- auto.
+- rewrite denotation_comp.
+  rewrite denotation_comp.
+  rewrite IHSC. reflexivity.
+- rewrite denotation_comp.
+  rewrite denotation_comp.
+  rewrite IHSC. reflexivity.
+- rewrite denotation_ite.
+  rewrite denotation_ite.
+  rewrite denotation_comp.
+  rewrite denotation_comp.
+  rewrite denotation_comp.
+  rewrite IHSC. reflexivity.
+- rewrite denotation_ite.
+  rewrite denotation_ite.
+  rewrite denotation_comp.
+  rewrite denotation_comp.
+  rewrite denotation_comp.
+  rewrite IHSC. reflexivity.
+- apply denotation_while_compat. auto.
+Qed.
+
+Lemma full_abstraction (S1: program):
+  bigstep_denotation S1 = denotation S1.
+Admitted.
+
+Lemma denotation_or (S: program) (X1 X2: resultset) (os: option state):
+  denotation S (fun os : option state => X1 os \/ X2 os) os ->
+  denotation S X1 os \/ denotation S X2 os.
+intros. generalize dependent X1. generalize dependent X2. generalize dependent os. induction S; intros.
+- rewrite denotation_oper in H.
+  rewrite denotation_oper.
+  admit.
+- admit.
+- admit.
+- rewrite denotation_comp in H. unfold compose in H.
+  rewrite denotation_comp. unfold compose.
+  apply denotation_monotonic with (Y := fun os => denotation S1 X1 os \/ denotation S1 X2 os) in H.
+  apply IHS2 in H. auto.
+  intros. apply IHS1 in H0. auto.
+- rewrite denotation_ite in H.
+  destruct H.
+  rewrite denotation_comp in H. unfold compose in H.
+Admitted.
+
+Lemma denotation_stateset_or (S: program) (X1 X2: stateset) (os: option state):
+  denotation S (fun os : option state => exists s : state, os = Some s /\ (X1 s \/ X2 s)) os ->
+  denotation S X1 os \/ denotation S X2 os.
+intros.
+apply denotation_monotonic with (Y := fun os : option state => (stateset_to_resultset X1) os \/ (stateset_to_resultset X2) os) in H.
+apply denotation_or. auto.
+intros. unfold stateset_to_resultset.
+destruct H0. destruct H0. destruct H1.
+left. exists x. tauto.
+right. exists x. tauto.
+Qed.
+
+End AbstractSemantics.
+
+Section AbstractHoare.
+
+Variable state: Type.
+
+Definition spec: Type := (state -> Prop) * program * (state -> Prop).
+
+Inductive HS (Ax: spec -> Prop): spec -> Prop :=
+| HS_axiom (pSq: spec): Ax pSq -> HS Ax pSq
+| HS_skip (X: state -> Prop): HS Ax (X, skip, X)
+| HS_diverge (X: state -> Prop): HS Ax (X, diverge, fun _ => False)
+| HS_comp (X Y Z: state -> Prop) (S1 S2: program):
+    HS Ax (X, S1, Y) -> HS Ax (Y, S2, Z) -> HS Ax (X, comp S1 S2, Z)
+| HS_ite (X Y: state -> Prop) (T: test) (S1 S2: program):
+    HS Ax (X, comp (assert T) S1, Y) -> HS Ax (X, comp (assert_not T) S2, Y) ->
+    HS Ax (X, ite T S1 S2, Y)
+| HS_while (X Y: state -> Prop) (T: test) (S: program):
+    HS Ax (X, comp (assert T) S, X) -> HS Ax (X, assert_not T, Y) ->
+    HS Ax (X, while T S, Y)
+| HS_conseq (X X' Y Y': state -> Prop) (S: program):
+    (forall x, X' x -> X x) -> (forall x, Y x -> Y' x) ->
+    HS Ax (X, S, Y) -> HS Ax (X', S, Y').
+
+Definition satisfied (M: machine_model state) (pSq: spec): Prop :=
+match pSq with
+| (X, S1, Y) => forall os, denotation M S1 (stateset_to_resultset X) os -> exists s, os = Some s /\ Y s
+end.
+
+Lemma HS_satisfied (M: machine_model state) (Ax: spec -> Prop) (pSq: spec):
+  (forall pSq, Ax pSq -> satisfied M pSq) -> HS Ax pSq -> satisfied M pSq.
+intros G H. induction H; simpl; intros.
+- apply G. auto.
+- rewrite denotation_skip in H. unfold id in H.
+  unfold stateset_to_resultset in H. auto.
+- rewrite denotation_diverge in H. unfold cap_fail in H.
+  destruct H. unfold stateset_to_resultset in H. destruct H. destruct H.
+  rewrite H in H0. inversion H0.
+- unfold satisfied in IHHS1, IHHS2.
+  rewrite denotation_comp in H1. unfold compose in H1.
+  eapply denotation_monotonic in H1.
+  apply IHHS2. apply H1.
+  intros. apply IHHS1. auto.
+- unfold satisfied in IHHS1, IHHS2.
+  rewrite denotation_ite in H1. destruct H1.
+  apply IHHS1 in H1. auto.
+  apply IHHS2 in H1. auto.
+- rename S into S1.
+  rewrite denotation_while in H1. destruct H1. induction x.
+  + simpl in H1. rewrite denotation_diverge in H1. unfold cap_fail in H1.
+    destruct H1. unfold stateset_to_resultset in H1. destruct H1. destruct H1.
+    rewrite H1 in H2. inversion H2.
+  + simpl in H1. rewrite denotation_ite in H1. destruct H1.
+    * rewrite <- denotation_assoc in H1.
+      rewrite denotation_comp in H1. unfold compose in H1.
+      unfold satisfied in IHHS1.
+      eapply denotation_monotonic in H1. apply IHx. apply H1.
+      intros. apply IHHS1 in H2. unfold stateset_to_resultset. auto.
+    * unfold satisfied in IHHS2.
+      rewrite denotation_comp in H1. unfold compose in H1.
+      rewrite denotation_skip in H1. unfold id in H1.
+      apply IHHS2 in H1. auto.
+- unfold satisfied in IHHS.
+  eapply denotation_monotonic in H2.
+  apply IHHS in H2. destruct H2. destruct H2. exists x. constructor; auto.
+  intros. unfold stateset_to_resultset in H3. unfold stateset_to_resultset.
+  destruct H3. destruct H3. exists x. auto.
+(*- unfold satisfied in IHX1, IHX2.
+  pose proof H as G.
+  eapply denotation_monotonic in H. apply IHX1 in H.
+  eapply denotation_monotonic in G. apply IHX2 in G.
+  destruct H. destruct G. assert (x = x0).
+  enough (Some x = Some x0). inversion H1. reflexivity.
+  destruct H. destruct H0. rewrite <- H. rewrite <- H0. reflexivity.
+  exists x. constructor. destruct H; auto.
+  destruct H; destruct H0; constructor; auto; rewrite H1; auto.
+  intros. unfold stateset_to_resultset in H0. destruct H0.
+  unfold stateset_to_resultset. exists x. tauto.
+  intros. unfold stateset_to_resultset in H0. destruct H0.
+  unfold stateset_to_resultset. exists x. tauto.
+- unfold satisfied in IHX1, IHX2.
+  unfold stateset_to_resultset in H.
+  apply denotation_stateset_or in H. destruct H.
+  eapply denotation_monotonic in H. apply IHX1 in H.
+  destruct H. exists x. tauto. tauto.
+  eapply denotation_monotonic in H. apply IHX2 in H.
+  destruct H. exists x. tauto. tauto. *)
+Qed.
+
+Definition singleton (s: state): resultset :=
+fun os => os = Some s.
+
+Definition weakest_pre (M: machine_model state) (S1: program) (Y: state -> Prop): state -> Prop :=
+fun p => exists q, Y q /\ denotation M S1 (singleton p) (Some q).
+
+Inductive HS_weakest (M: machine_model state): spec -> Prop :=
+| weakest_HS (pSq: spec): HS (HS_weakest M) pSq -> HS_weakest M pSq
+| weakest_oper (o: op) (Y: state -> Prop): HS_weakest M (weakest_pre M (oper o) Y, oper o, Y).
+
+
+
+
+
+
+
+
+
+
